Adding a type t_exact supported by the `t x[=size]` notation

src/3d/ocaml/lexer.mll
@@ -100,6 +100,7 @@ rule token =
   | "{:on-success" { locate lexbuf LBRACE_ONSUCCESS }
   | "{"            { locate lexbuf LBRACE }
   | "}"            { locate lexbuf RBRACE }
+  | "[="           { locate lexbuf LBRACK_EQ }    
   | "[<="          { locate lexbuf LBRACK_LEQ }  
   | "["            { locate lexbuf LBRACK }
   | "]"            { locate lexbuf RBRACK }  
