src/3d/prelude/Actions.fst
@@ -887,6 +887,36 @@ let validate_t_at_most (n:U32.t) (#k:parser_kind true) (#t:_) (#p:parser k t)
         in
         startPosition `U64.add` Cast.uint32_to_uint64 n
 
+[@ CMacro ]
+let validator_error_unexpected_padding : LPL.validator_error = normalize_term (LPL.set_validator_error_kind 0uL 7uL)
+
+noextract inline_for_extraction
+let validate_t_exact (n:U32.t) (#k:parser_kind true) (#t:_) (#p:parser k t)
+                       (#inv:_) (#l:_) (#ar:_) (v:validate_with_action_t p inv l ar)
+  : Tot (validate_with_action_t (parse_t_exact n p) inv l false)
+  = fun input startPosition ->
+    let h = HST.get () in
+    let _ =
+      LPL.valid_weaken kind_t_at_most (LowParse.Spec.FLData.parse_fldata p (U32.v n)) h input (LPL.uint64_to_uint32 startPosition);
+      LPL.valid_facts (LowParse.Spec.FLData.parse_fldata p (U32.v n)) h input (LPL.uint64_to_uint32 startPosition)
+    in
+    if (Cast.uint32_to_uint64 input.LPL.len `U64.sub` startPosition) `U64.lt` Cast.uint32_to_uint64 n
+    then LPL.validator_error_not_enough_data
+    else
+      [@inline_let] let input' = { LPL.base = input.LPL.base; LPL.len = LPL.uint64_to_uint32 startPosition `U32.add` n; } in
+      [@inline_let] let _ =
+        LPL.valid_facts p h input' (LPL.uint64_to_uint32 startPosition)
+      in
+      // FIXME: I'd need a name here
+      let positionAfterContents = v input' startPosition in
+      let h1 = HST.get () in
+      let _ = modifies_address_liveness_insensitive_unused_in h h1 in
+      if LPL.is_error positionAfterContents
+      then positionAfterContents
+      else if (LPL.uint64_to_uint32 positionAfterContents) <> input'.LPL.len
+      then validator_error_unexpected_padding
+      else startPosition `U64.add` Cast.uint32_to_uint64 n
+
 
 inline_for_extraction noextract
 let validate_with_comment (c:string)
