src/3d/Ast.fst
@@ -252,9 +252,10 @@ and bitfield_attr = with_meta_t bitfield_attr'
 let field_bitwidth_t = either (with_meta_t int) bitfield_attr
 
 type array_qualifier =
-  | VariableSizeEq
-  | VariableSizeLeq
-  | ConstantSize
+  | VariableSizeEq              //[Size]
+  | VariableSizeLeq             //[<= Size]
+  | SingleElementVariableSizeEq //[= Size]
+  | ConstantSize                //[N]
 
 noeq
 type struct_field = {
@@ -540,6 +541,7 @@ let print_field (f:field) : ML string =
     match q with
     | VariableSizeEq -> Printf.sprintf "[%s]" (print_expr e)
     | VariableSizeLeq -> Printf.sprintf "[<= %s]" (print_expr e)
+    | SingleElementVariableSizeEq -> Printf.sprintf "[= %s]" (print_expr e)
     | ConstantSize -> Printf.sprintf "[{ %s }]" (print_expr e)
   in
   let sf = f.v in
